rocq/theories/TypeSystem/TypeSafetyHiddenFrameBase.v
@@ -276,6 +276,127 @@ Definition captured_call_frame_params_ready
   captured_call_frame_ready env captured Rcap s_args R_args /\
   captured_params_store_typed env captured caps.
 
+Fixpoint copy_capture_roots_as
+    (captures : list ident) (caps : list param) (R : root_env)
+    : option root_env :=
+  match captures, caps with
+  | [], [] => Some []
+  | x :: captures', cap :: caps' =>
+      match root_env_lookup x R, copy_capture_roots_as captures' caps' R with
+      | Some roots, Some Rcap =>
+          Some ((param_name cap, roots) :: Rcap)
+      | _, _ => None
+      end
+  | _, _ => None
+  end.
+
+Lemma copy_capture_roots_as_length :
+  forall captures caps R Rcap,
+    copy_capture_roots_as captures caps R = Some Rcap ->
+    List.length captures = List.length caps.
+Proof.
+  intros captures.
+  induction captures as [| x captures IH]; intros caps R Rcap Hcopy;
+    destruct caps as [| cap caps]; simpl in Hcopy; try discriminate;
+    simpl.
+  - reflexivity.
+  - destruct (root_env_lookup x R) as [roots |] eqn:Hlookup;
+      try discriminate.
+    destruct (copy_capture_roots_as captures caps R) as [Rtail |]
+      eqn:Htail; try discriminate.
+    injection Hcopy as <-.
+    f_equal. eapply IH. exact Htail.
+Qed.
+
+Lemma copy_capture_roots_as_names :
+  forall captures caps R Rcap,
+    copy_capture_roots_as captures caps R = Some Rcap ->
+    root_env_names Rcap = ctx_names (params_ctx caps).
+Proof.
+  intros captures.
+  induction captures as [| x captures IH]; intros caps R Rcap Hcopy;
+    destruct caps as [| cap caps]; simpl in Hcopy; try discriminate.
+  - injection Hcopy as <-. reflexivity.
+  - destruct (root_env_lookup x R) as [roots |] eqn:Hlookup;
+      try discriminate.
+    destruct (copy_capture_roots_as captures caps R) as [Rtail |]
+      eqn:Htail; try discriminate.
+    injection Hcopy as <-.
+    simpl. rewrite (IH caps R Rtail Htail). reflexivity.
+Qed.
+
+Lemma copy_capture_roots_as_no_shadow :
+  forall captures caps R Rcap,
+    copy_capture_roots_as captures caps R = Some Rcap ->
+    NoDup (ctx_names (params_ctx caps)) ->
+    root_env_no_shadow Rcap.
+Proof.
+  intros captures caps R Rcap Hcopy Hnodup.
+  unfold root_env_no_shadow.
+  rewrite (copy_capture_roots_as_names captures caps R Rcap Hcopy).
+  exact Hnodup.
+Qed.
+
+Lemma param_name_nth_error_in_params_ctx :
+  forall caps n cap,
+    nth_error caps n = Some cap ->
+    In (param_name cap) (ctx_names (params_ctx caps)).
+Proof.
+  induction caps as [| cap0 caps IH]; intros n cap Hnth;
+    destruct n as [| n]; simpl in Hnth; try discriminate.
+  - injection Hnth as <-. simpl. left. reflexivity.
+  - simpl. right. eapply IH. exact Hnth.
+Qed.
+
+Lemma copy_capture_roots_as_lookup_nth :
+  forall captures caps R Rcap n src cap roots,
+    copy_capture_roots_as captures caps R = Some Rcap ->
+    NoDup (ctx_names (params_ctx caps)) ->
+    nth_error captures n = Some src ->
+    nth_error caps n = Some cap ->
+    root_env_lookup src R = Some roots ->
+    root_env_lookup (param_name cap) Rcap = Some roots.
+Proof.
+  intros captures.
+  induction captures as [| x captures IH];
+    intros caps R Rcap n src cap roots Hcopy Hnodup Hsrc Hcap Hlookup_src;
+    destruct caps as [| cap0 caps]; simpl in Hcopy; try discriminate.
+  - destruct n; simpl in Hsrc; discriminate.
+  - destruct (root_env_lookup x R) as [roots0 |] eqn:Hlookup_x;
+      try discriminate.
+    destruct (copy_capture_roots_as captures caps R) as [Rtail |]
+      eqn:Htail; try discriminate.
+    injection Hcopy as <-.
+    destruct n as [| n].
+    + simpl in Hsrc, Hcap.
+      injection Hsrc as <-. injection Hcap as <-.
+      rewrite Hlookup_src in Hlookup_x. injection Hlookup_x as <-.
+      simpl. rewrite ident_eqb_refl. reflexivity.
+    + simpl in Hsrc, Hcap.
+      simpl.
+      inversion Hnodup as [| ? ? Hnotin Hnodup_tail]; subst.
+      destruct (ident_eqb (param_name cap) (param_name cap0)) eqn:Heq.
+      * apply ident_eqb_eq in Heq.
+        exfalso.
+        apply Hnotin.
+        rewrite <- Heq.
+        eapply param_name_nth_error_in_params_ctx. exact Hcap.
+      * eapply IH; eassumption.
+Qed.
+
+Lemma copy_capture_roots_as_lookup_head :
+  forall x captures cap caps R Rcap roots,
+    copy_capture_roots_as (x :: captures) (cap :: caps) R = Some Rcap ->
+    NoDup (ctx_names (params_ctx (cap :: caps))) ->
+    root_env_lookup x R = Some roots ->
+    root_env_lookup (param_name cap) Rcap = Some roots.
+Proof.
+  intros x captures cap caps R Rcap roots Hcopy Hnodup Hlookup.
+  eapply copy_capture_roots_as_lookup_nth with
+    (captures := x :: captures) (caps := cap :: caps)
+    (n := 0) (src := x) (cap := cap); eauto.
+Qed.
+
 Lemma check_make_closure_captures_exact_sctx_sound :
   forall env Ω Σ captures caps captured_tys,
     check_make_closure_captures_exact_sctx env Ω Σ captures caps =
@@ -326,6 +447,82 @@ Proof.
       * apply ty_compatible_refl.
       * exact Htyped_tail.
     + simpl. rewrite Htys_tail. reflexivity.
+Qed.
+
+Lemma check_make_closure_captures_exact_sctx_with_env_base_sound :
+  forall env Ω Σ captures caps captured_tys env_lt,
+    check_make_closure_captures_exact_sctx_with_env_base
+      env Ω Σ captures caps = infer_ok captured_tys ->
+    closure_captures_allowed_b env Ω env_lt captured_tys = true ->
+    typed_captures Ω Σ env_lt captures caps captured_tys /\
+    captured_tys = map param_ty caps.
+Proof.
+  intros env Ω Σ captures.
+  induction captures as [| x captures IH]; intros caps captured_tys env_lt
+    Hcheck Hallowed;
+    destruct caps as [| cap caps]; simpl in Hcheck; try discriminate.
+  - injection Hcheck as <-.
+    split; constructor.
+  - destruct (param_mutability cap) eqn:Hcap_mut; simpl in Hcheck;
+      try discriminate.
+    destruct (sctx_lookup (param_name cap) Σ) as [[Tcap stcap] |]
+      eqn:Hcap_lookup; try discriminate.
+    destruct (sctx_lookup x Σ) as [[T st] |] eqn:Hlookup; try discriminate.
+    destruct (st_consumed st) eqn:Hconsumed; try discriminate.
+    destruct (st_moved_paths st) as [| moved moved_rest] eqn:Hmoved;
+      try discriminate.
+    destruct (sctx_lookup_mut x Σ) as [m |] eqn:Hmut; try discriminate.
+    destruct m; try discriminate.
+    destruct (usage_eqb (ty_usage T) UUnrestricted) eqn:Husage;
+      try discriminate.
+    destruct (ty_eqb T (param_ty cap) &&
+      ty_compatible_b Ω T (param_ty cap)) eqn:Hty; try discriminate.
+    apply andb_true_iff in Hty as [Hty_eq Hcompat].
+    destruct (check_make_closure_captures_exact_sctx_with_env_base
+      env Ω Σ captures caps) as [captured_rest | err] eqn:Hrest;
+      try discriminate.
+    injection Hcheck as <-.
+    simpl in Hallowed.
+    apply andb_true_iff in Hallowed as [Hallowed_head Hallowed_tail].
+    destruct (IH caps captured_rest env_lt Hrest Hallowed_tail)
+      as [Htyped_tail Htys_tail].
+    assert (Havailable : binding_available_b st [] = true).
+    { unfold binding_available_b.
+      rewrite Hconsumed, Hmoved. reflexivity. }
+    assert (HTeq : T = param_ty cap).
+    { apply ty_eqb_true. exact Hty_eq. }
+    subst T.
+    split.
+    + eapply TCap_Cons.
+      * unfold sctx_lookup in Hlookup.
+        eapply ctx_lookup_state_available_nil_lookup; eassumption.
+      * exact Hmut.
+      * apply usage_eqb_true. exact Husage.
+      * eapply closure_capture_allowed_b_sound. exact Hallowed_head.
+      * apply ty_compatible_b_sound. exact Hcompat.
+      * exact Htyped_tail.
+    + simpl. rewrite Htys_tail. reflexivity.
+Qed.
+
+Lemma check_make_closure_captures_exact_sctx_with_env_sound :
+  forall env Ω Σ captures caps env_lt captured_tys,
+    check_make_closure_captures_exact_sctx_with_env env Ω Σ captures caps =
+      infer_ok (env_lt, captured_tys) ->
+    typed_captures Ω Σ env_lt captures caps captured_tys /\
+    captured_tys = map param_ty caps.
+Proof.
+  intros env Ω Σ captures caps env_lt captured_tys Hcheck.
+  unfold check_make_closure_captures_exact_sctx_with_env in Hcheck.
+  destruct (check_make_closure_captures_exact_sctx_with_env_base
+    env Ω Σ captures caps) as [captured_tys0 | err] eqn:Hbase;
+    try discriminate.
+  destruct (infer_closure_env_lifetime Ω captured_tys0) as [env_lt0 | err]
+    eqn:Henv; try discriminate.
+  destruct (closure_captures_allowed_b env Ω env_lt0 captured_tys0)
+    eqn:Hallowed; try discriminate.
+  injection Hcheck as <- <-.
+  eapply check_make_closure_captures_exact_sctx_with_env_base_sound;
+    eassumption.
 Qed.
 
 Lemma binding_available_nil_fresh :
